#Processed by Id: cwm.py,v 1.93 2002/05/14 22:11:04 timbl Exp 
        #    using base file:/devel/WWW/2000/10/swap/db.n3
        
#  Notation3 generation by
#       notation3.py,v 1.108 2002/05/15 00:38:10 timbl Exp

#   Base was: file:/devel/WWW/2000/10/swap/db.n3
     @prefix : <http://www.w3.org/2000/10/swap/db#> .
     @prefix con: <http://www.w3.org/2000/10/swap/pim/contact#> .
     @prefix daml: <http://www.daml.org/2001/03/daml+oil#> .
     @prefix dc: <http://purl.org/dc/elements/1.1/> .
     @prefix doc: <http://www.w3.org/2000/10/swap/pim/doc#> .
     @prefix log: <http://www.w3.org/2000/10/swap/log#> .
     @prefix rdf: <http://www.w3.org/1999/02/22-rdf-syntax-ns#> .
     @prefix rdfs: <http://www.w3.org/2000/01/rdf-schema#> .
    
    <>     <http://purl.org/dc/elements/1.1/creator>  [
             con:mailbox <mailto:timbl@w3.org> ],
                 [
             con:mailbox <mailto:connolly@w3.org> ];
         <http://purl.org/dc/elements/1.1/description> """
Note that table documents are namespace documents: when you
define a prefix to correspond to the table document's URI with a hash on,
then the table document automatically an RDF schema for the namespace. 
""";
         <http://purl.org/dc/elements/1.1/title> "Database terms for the Sematic Web";
         doc:version "$Id$" .
    
    :Column     a rdfs:Class;
         rdfs:comment "A property corresponding to a database column name.";
         rdfs:label "column";
         rdfs:subClassOf rdf:Property .
    
    :Database     a rdfs:Class;
         rdfs:comment " ";
         rdfs:label "database" .
    
    :DatabaseDocument     a rdfs:Class;
         rdfs:comment """The resource on the web which describes a database, though not
    the one which contains all the data.
    Convention: Any database <xxx#f> has a databaseDocumemnt <xxx>.""";
         rdfs:label "database document";
         rdfs:subClassOf doc:Work .
    
    :RowDocument     a rdfs:Class;
         rdfs:comment """A row document exists for each row of a table which 
has a primary key.  Its URI is formed by convention by concatenating the
the URI of the table, a slash, and the URI-encoded value of the
primary key value for that row. 

The row document gives the value of each cell in the row.
It identifies the row with a local <#item> URI.
It must also identify <#item> as being of rdf$type of the Table.
""";
         rdfs:label "row document";
         rdfs:subClassOf doc:Work .
    
    :Table     a rdfs:Class;
         rdfs:comment """A Table is a class which has in it a finite
    set of things each of which is described by a row in the database table""";
         rdfs:label "Table";
         rdfs:subClassOf rdfs:Class .
    
    :TableDocument     a rdfs:Class;
         rdfs:comment """The resource on the web which describes a Table, though not
    the one which contains all the data.
    Convention: Any table <xxx#f> has a tabledocumemnt <xxx>.

   The table document defines a set of db:Column's, one for each column
   of the table.  It is definitive, in that any column in the table MUST
   be described in the table document.

   The table document must also give the database document for the databse the table
   is in.  It is sufficent to quote the URI of the database, as the database document's
   URI follows from the convention.
   This allows a client application to find the other properties of the database.
""";
         rdfs:label "table document";
         rdfs:subClassOf doc:Work .
    
    :column     a rdf:Property;
         rdfs:comment """The relationship between a table and one of its columns.

The fact that a table has a db:column in this sense assures that certain conventions
are followed.
1. For any Column <xxx#f> there is always a corresponding table document <xxx>
    which defines it (i.e. says something about it, at least that it is a colmn of the
    table).
""";
         rdfs:domain :Table;
         rdfs:label "column";
         rdfs:range :Column .
    
    :databaseSchema     a rdf:Property;
         rdfs:comment "The document which describes the form of this database";
         rdfs:domain :Database;
         rdfs:label "database schema";
         rdfs:range :DatabaseDocument .
    
    :primaryKey     a daml:UniqueProperty;
         rdfs:comment """
The fact that a table has primary key means that a row document exists
whose URI is formed by concatenating the URI of the table, a slash, and
the URI-encoded value of the primary key value for that row.
""";
         rdfs:range daml:UnambiguousProperty;
         rdfs:subPropertyOf :column .
    
    :table     a rdf:Property;
         rdfs:comment "A table in the database";
         rdfs:domain :Database;
         rdfs:label "table";
         rdfs:range :Table .
    
    :tableData     a rdf:Property;
         rdfs:comment "The document which gives the data in this table";
         rdfs:domain :Table;
         rdfs:label "table data";
         rdfs:range doc:Work .
    
    :tableSchema     a rdf:Property;
         rdfs:comment "The document which describes the form of this table";
         rdfs:domain :Table;
         rdfs:label "table schema";
         rdfs:range :TableDocument .
    
#ENDS
