
<!-- Processed by Id: cwm.py,v 1.121 2003/02/02 16:09:06 timbl Exp -->
<!--     using base file:/devel/WWW/2000/10/swap/log.n3-->


<rdf:RDF xmlns="http://www.w3.org/2000/10/swap/log#"
    xmlns:doc="http://www.w3.org/2000/10/swap/pim/doc#"
    xmlns:log="http://www.w3.org/2000/10/swap/log#"
    xmlns:rdf="http://www.w3.org/1999/02/22-rdf-syntax-ns#"
    xmlns:rdfs="http://www.w3.org/2000/01/rdf-schema#">

    <rdfs:Class rdf:about="http://www.w3.org/2000/10/swap/log#Chaff">
        <rdfs:comment>Any statement mentioning anything in this class
is considered boring and purged by the cwm --purge option.
This is a convenience, and does not have any value when published as a
general fact on the web.</rdfs:comment>
    </rdfs:Class>

    <rdfs:Class rdf:about="http://www.w3.org/2000/10/swap/log#Formula">
    </rdfs:Class>

    <rdfs:Class rdf:about="http://www.w3.org/2000/10/swap/log#List">
    </rdfs:Class>

    <rdfs:Class rdf:about="http://www.w3.org/2000/10/swap/log#N3Document">
        <rdfs:comment>A document which, which parsed as Notation3
as defined in general by http://www.w3.org/DesignIssues/Notation3.html
and this schema, conveys the intent of the author by the semantics defined
on those specifications, and the semantics defined by the specifications
of any identifiers used in the document.
</rdfs:comment>
    </rdfs:Class>

    <rdfs:Class rdf:about="http://www.w3.org/2000/10/swap/log#Other">
    </rdfs:Class>

    <rdfs:Class rdf:about="http://www.w3.org/2000/10/swap/log#String">
    </rdfs:Class>

    <rdfs:Class rdf:about="http://www.w3.org/2000/10/swap/log#Truth">
        <rdfs:comment>Something which is true: belive it as you would belive this.
	       Understood natively by cwm in that it will execute rules in a formula
         declared a Truth within a formula it is already taking rules from.</rdfs:comment>
    </rdfs:Class>

    <rdf:Property rdf:about="http://www.w3.org/2000/10/swap/log#conclusion">
        <rdfs:comment>All possible conclusions which can be drawn from a formula.

The object of this function is the set of conclusions which can be
drawn from the subject formula, by successively applying any
rules it contains to the data it contains. This is equivalent to
cwm's "--think" command line function.  It does use built-ins, so
it may for example indirectly invoke other documents, validate
signatures, etc.
</rdfs:comment>
        <rdfs:domain rdf:resource="http://www.w3.org/2000/10/swap/log#Formula"/>
        <rdfs:label>conclusion</rdfs:label>
        <rdfs:range rdf:resource="http://www.w3.org/2000/10/swap/log#Formula"/>
    </rdf:Property>

    <rdf:Property rdf:about="http://www.w3.org/2000/10/swap/log#conjunction">
        <rdfs:comment>"A function to merge formulae: logical AND.

The subject is a list of formulae.
The object, which can be generated, is a formula containing a copy
of each of the formulae in the list on the left.
A cwm built-in function.
</rdfs:comment>
        <rdfs:domain rdf:resource="http://www.w3.org/2000/10/swap/log#List"/>
        <rdfs:label>conjunction</rdfs:label>
        <rdfs:range rdf:resource="http://www.w3.org/2000/10/swap/log#Formula"/>
    </rdf:Property>

    <rdf:Property rdf:about="http://www.w3.org/2000/10/swap/log#content">
        <rdfs:comment>This connects a document and a string that represents it.
        Cwm knows how to go get a document in order to evaluate this.</rdfs:comment>
        <rdfs:domain rdf:resource="http://www.w3.org/2000/10/swap/pim/doc#Work"/>
        <rdfs:label>content</rdfs:label>
        <rdfs:range rdf:resource="http://www.w3.org/2000/10/swap/log#String"/>
    </rdf:Property>

    <rdf:Property rdf:about="http://www.w3.org/2000/10/swap/log#definitiveDocument">
        <rdfs:comment>	When document D is the definitiveDocument for property P,
any statement X P Y is true iff and only if the semantics of document D
include that statement.

For example, there may be a definitive document for the zipcode of
airports by airport code, and so on. This is useful to let a reasoner
know that it can extend its query to the given document.
(Cwm will do this if its mode includes "r").
</rdfs:comment>
        <rdfs:domain rdf:resource="http://www.w3.org/1999/02/22-rdf-syntax-ns#Property"/>
        <rdfs:label>definitive document</rdfs:label>
        <rdfs:range rdf:resource="http://www.w3.org/2000/10/swap/pim/doc#Work"/>
    </rdf:Property>

    <rdf:Property rdf:about="http://www.w3.org/2000/10/swap/log#definitiveService">
        <rdfs:comment>	When service S is the definitiveService for property P,
any statement X P Y is true iff and only if a query to S returns
that it is.  The protocol for the service S depends on the scheme.
For mysql protocol, the URI of the service is like
sql://user:password@host.domain/database/.

For example, there may be a definitive service for the zipcode of
airports by airport code, and so on. This is useful to let a reasoner
know that it can help resolve a query by delegating it to the service
in question.
(Cwm will do this if its mode includes "r").
</rdfs:comment>
        <rdfs:domain rdf:resource="http://www.w3.org/1999/02/22-rdf-syntax-ns#Property"/>
        <rdfs:label>definitive service</rdfs:label>
    </rdf:Property>

    <rdf:Property rdf:about="http://www.w3.org/2000/10/swap/log#equalTo">
        <rdfs:comment>Equality in this sense is actually the same URI.
Do not confuse with daml:EquivalentTo.
A cwm built-in logical operator.
</rdfs:comment>
    </rdf:Property>

    <SyntaxArc rdf:about="http://www.w3.org/2000/10/swap/log#forAll">
        <rdfs:comment>A is true for any object in place of B.</rdfs:comment>
        <rdfs:label>for All</rdfs:label>
    </SyntaxArc>

    <rdf:SyntaxArc rdf:about="http://www.w3.org/2000/10/swap/log#forSome">
        <rdfs:comment>A is true for some object for which here we use B. This
        is NOT a real rdf property in its behaviour - a pseudoproperty.
	For example, removal of it from a formula does nor
	preserve truth, and substitution is not permitted on its object.</rdfs:comment>
        <rdfs:domain rdf:resource="http://www.w3.org/2000/10/swap/log#Formula"/>
    </rdf:SyntaxArc>

    <rdf:Property rdf:about="http://www.w3.org/2000/10/swap/log#implies">
        <rdfs:comment>Logical implication. Understood natively by cwm.</rdfs:comment>
        <rdfs:isDefinedBy rdf:resource=""/>
        <rdfs:range rdf:resource="http://www.w3.org/2000/10/swap/log#Formula"/>
    </rdf:Property>

    <rdf:Property rdf:about="http://www.w3.org/2000/10/swap/log#includes">
        <rdfs:comment>One formula is subset of other. Understood natively by cwm.</rdfs:comment>
        <rdfs:isDefinedBy rdf:resource=""/>
        <rdfs:range rdf:resource="http://www.w3.org/2000/10/swap/log#Formula"/>
    </rdf:Property>

    <rdf:Property rdf:about="http://www.w3.org/2000/10/swap/log#notEqualTo">
        <rdfs:comment>Equality in this sense is actually the same URI.
Do not confuse with daml:EquivalentTo.
A cwm built-in logical operator.
</rdfs:comment>
    </rdf:Property>

    <rdf:Property rdf:about="http://www.w3.org/2000/10/swap/log#notIncludes">
        <rdfs:comment>One formula is NOT a subset of other. Understood natively by cwm.</rdfs:comment>
        <rdfs:isDefinedBy rdf:resource=""/>
        <rdfs:range rdf:resource="http://www.w3.org/2000/10/swap/log#Formula"/>
    </rdf:Property>

    <rdf:Property rdf:about="http://www.w3.org/2000/10/swap/log#outputString">
        <rdfs:comment>The subject is a key and the object is a string,
where the strings are to be output in the order of the keys.
See cwm --strings in cwm --help.
</rdfs:comment>
        <rdfs:label>output string</rdfs:label>
    </rdf:Property>

    <rdf:Property rdf:about="http://www.w3.org/2000/10/swap/log#parsedAsN3">
        <rdfs:comment>A string, parsed as N3, gives this formula.</rdfs:comment>
        <rdfs:domain rdf:resource="http://www.w3.org/2000/10/swap/log#String"/>
        <rdfs:label>parses to</rdfs:label>
        <rdfs:range rdf:resource="http://www.w3.org/2000/10/swap/log#Formula"/>
    </rdf:Property>

    <rdf:Property rdf:about="http://www.w3.org/2000/10/swap/log#racine">
        <rdfs:comment>For anything identified by a URI with a fragid, this is the
        thing identified by the same URI without a hash or fragid</rdfs:comment>
    </rdf:Property>

    <rdf:Property rdf:about="http://www.w3.org/2000/10/swap/log#rawType">
        <rdfs:comment>
This is a low-level langauge type, one of log:Formula, log:Literal, 
log:List, log:Other.  I only use testing for log:Formula right now (tbl 2001/9/17).
List and Other are not stable and may change.
Example: semanticsOrError returns either a Formula or a String.
</rdfs:comment>
    </rdf:Property>

    <rdf:Property rdf:about="http://www.w3.org/2000/10/swap/log#semantics">
        <rdfs:comment>This connects a document and the formula it parses to.
        Cwm knows how to go get a document and parse it in order to evaluate this.</rdfs:comment>
        <rdfs:domain rdf:resource="http://www.w3.org/2000/10/swap/pim/doc#Work"/>
        <rdfs:label>semantics</rdfs:label>
        <rdfs:range rdf:resource="http://www.w3.org/2000/10/swap/log#Formula"/>
    </rdf:Property>

    <rdf:Property rdf:about="http://www.w3.org/2000/10/swap/log#semanticsOrError">
        <rdfs:comment>This connects a document and either the formula it parses to,
        or an error message explaining what went wromg with trying. See semantics.
        Cwm knows how to go get a document and parse it in order to evaluate this.</rdfs:comment>
        <rdfs:domain rdf:resource="http://www.w3.org/2000/10/swap/pim/doc#Work"/>
        <rdfs:label>semantics or error message</rdfs:label>
    </rdf:Property>

    <rdf:Property rdf:about="http://www.w3.org/2000/10/swap/log#uri">
        <rdfs:comment>This allows one to look at the actual string of the URI which identifies this.

Cwm can get the URI of a resource or get the resource from the URI.
This is a level breaker, breaking the rule of not looking inside a
URI.   Use (eg with  string:match) to replace RDF's old "aboutEach" functionality.</rdfs:comment>
        <rdfs:range rdf:resource="http://www.w3.org/2000/10/swap/log#String"/>
    </rdf:Property>
</rdf:RDF>
