
<!-- Processed by Id: cwm.py,v 1.121 2003/02/02 16:09:06 timbl Exp -->
<!--     using base file:/devel/WWW/2000/10/swap/math.n3-->


<rdf:RDF xmlns="http://www.w3.org/2000/10/swap/math#"
    xmlns:daml="http://www.daml.org/2001/03/daml+oil#"
    xmlns:log="http://www.w3.org/2000/10/swap/log#"
    xmlns:math="http://www.w3.org/2000/10/swap/math#"
    xmlns:rdf="http://www.w3.org/1999/02/22-rdf-syntax-ns#"
    xmlns:rdfs="http://www.w3.org/2000/01/rdf-schema#"
    xmlns:string="http://www.w3.org/2000/10/swap/string#">

    <rdfs:Class rdf:about="http://www.w3.org/2000/10/swap/math#Function">
        <rdfs:comment>A math:Function is unique in terms of math:EqualTo. </rdfs:comment>
        <rdfs:label>Function</rdfs:label>
        <rdfs:subClassOf rdf:resource="http://www.w3.org/1999/02/22-rdf-syntax-ns#Property"/>
    </rdfs:Class>

    <rdfs:Class rdf:about="http://www.w3.org/2000/10/swap/math#List">
        <rdfs:comment>The class of things that are DAML lists were all of the 
      members are math:Value items.</rdfs:comment>
        <rdfs:label>List</rdfs:label>
        <rdfs:subClassOf rdf:resource="http://www.daml.org/2001/03/daml+oil#List"/>
    </rdfs:Class>

    <rdfs:Class rdf:about="http://www.w3.org/2000/10/swap/math#LogicalOperator">
        <rdfs:comment>a logical operator allows evaluation eihter way, or testing relationship
         between two values</rdfs:comment>
        <rdfs:subClassOf rdf:resource="http://www.w3.org/2000/10/swap/math#Function"/>
        <rdfs:subClassOf rdf:resource="http://www.w3.org/2000/10/swap/math#ReverseFunction"/>
    </rdfs:Class>

    <rdfs:Class rdf:about="http://www.w3.org/2000/10/swap/math#ReverseFunction">
        <rdfs:comment>A math:ReverseFunction is unambiguous in terms of math:EqualTo. </rdfs:comment>
        <rdfs:subClassOf rdf:resource="http://www.w3.org/1999/02/22-rdf-syntax-ns#Property"/>
    </rdfs:Class>

    <rdfs:Class rdf:about="http://www.w3.org/2000/10/swap/math#StrictProperty">
        <rdfs:label>StrictProperty</rdfs:label>
        <rdfs:subClassOf rdf:resource="http://www.w3.org/1999/02/22-rdf-syntax-ns#Property"/>
    </rdfs:Class>

    <rdfs:Class rdf:about="http://www.w3.org/2000/10/swap/math#TwoMemberedList">
        <rdfs:comment>This is the class of things that are math lists with only two members.</rdfs:comment>
        <rdfs:label>TwoMemberedList</rdfs:label>
        <rdfs:subClassOf rdf:resource="http://www.w3.org/2000/10/swap/math#List"/>
    </rdfs:Class>

    <rdfs:Class rdf:about="http://www.w3.org/2000/10/swap/math#Value">
        <rdfs:comment>The class of things that are numeric float values as in Python.</rdfs:comment>
        <rdfs:label>Value</rdfs:label>
        <rdfs:subClassOf rdf:resource="http://www.w3.org/2000/10/swap/string#String"/>
    </rdfs:Class>

    <rdf:Property rdf:about="http://www.w3.org/2000/10/swap/math#absoluteValue">
        <rdfs:comment>The object is calulated as the absolute value of the subject.</rdfs:comment>
        <rdfs:domain rdf:resource="http://www.w3.org/2000/10/swap/math#Value"/>
        <rdfs:label>negation</rdfs:label>
        <rdfs:range rdf:resource="http://www.w3.org/2000/10/swap/math#Value"/>
    </rdf:Property>

    <rdf:Property rdf:about="http://www.w3.org/2000/10/swap/math#difference">
        <rdfs:comment>The subject is a pair of numbers. The object
is calculated by dividing the first number of the pair by the second.
</rdfs:comment>
        <rdfs:comment>The subject is a pair of numbers. The object
is calculated by subtracting the second number of the pair from the first.
</rdfs:comment>
        <rdfs:label>difference</rdfs:label>
        <rdfs:range rdf:resource="http://www.w3.org/2000/10/swap/math#Value"/>
    </rdf:Property>

    <ReverseFunction rdf:about="http://www.w3.org/2000/10/swap/math#differenceOf">
        <rdfs:comment>The difference of the list members. (obsolete)</rdfs:comment>
        <rdfs:domain rdf:resource="http://www.w3.org/2000/10/swap/math#Value"/>
        <rdfs:label>differenceOf</rdfs:label>
        <rdfs:range rdf:resource="http://www.w3.org/2000/10/swap/math#TwoMemberedList"/>
    </ReverseFunction>

    <StrictProperty rdf:about="http://www.w3.org/2000/10/swap/math#equalTo">
        <rdfs:comment>True iff the subject is a string representation of a number which  is EQUAL TO a number of which the object is a string representation.</rdfs:comment>
        <rdfs:domain rdf:resource="http://www.w3.org/2000/10/swap/math#Value"/>
        <rdfs:label>equalTo</rdfs:label>
        <rdfs:range rdf:resource="http://www.w3.org/2000/10/swap/math#Value"/>
    </StrictProperty>

    <rdf:Property rdf:about="http://www.w3.org/2000/10/swap/math#exponentiation">
        <rdfs:comment>The subject is a pair of numbers. The object
is calculated by raising the first number of the power of the second.
</rdfs:comment>
        <rdfs:label>exponentiation</rdfs:label>
        <rdfs:range rdf:resource="http://www.w3.org/2000/10/swap/math#Value"/>
    </rdf:Property>

    <ReverseFunction rdf:about="http://www.w3.org/2000/10/swap/math#exponentiationOf">
        <rdfs:comment>For exponOf(x, (y, z)), x = y^z   (obsolete)</rdfs:comment>
        <rdfs:domain rdf:resource="http://www.w3.org/2000/10/swap/math#Value"/>
        <rdfs:label>exponentiationOf</rdfs:label>
        <rdfs:range rdf:resource="http://www.w3.org/2000/10/swap/math#TwoMemberedList"/>
    </ReverseFunction>

    <ReverseFunction rdf:about="http://www.w3.org/2000/10/swap/math#factors">
        <daml:inverse rdf:resource="http://www.w3.org/2000/10/swap/math#product"/>
        <rdfs:comment>A list of values which multiply to produce the subject. (obsolete)</rdfs:comment>
        <rdfs:domain rdf:resource="http://www.w3.org/2000/10/swap/math#Value"/>
        <rdfs:label>factors</rdfs:label>
        <rdfs:range rdf:resource="http://www.w3.org/2000/10/swap/math#List"/>
    </ReverseFunction>

    <StrictProperty rdf:about="http://www.w3.org/2000/10/swap/math#greaterThan">
        <rdfs:comment>True iff the subject is a string representation of a number which  is greater than the number of which the object is a string representation.</rdfs:comment>
        <rdfs:domain rdf:resource="http://www.w3.org/2000/10/swap/math#Value"/>
        <rdfs:label>greaterThan</rdfs:label>
        <rdfs:range rdf:resource="http://www.w3.org/2000/10/swap/math#Value"/>
    </StrictProperty>

    <StrictProperty rdf:about="http://www.w3.org/2000/10/swap/math#lessThan">
        <rdfs:comment>True iff the subject is a string representation of a number which  is LESS than a number of which the object is a string representation.</rdfs:comment>
        <rdfs:domain rdf:resource="http://www.w3.org/2000/10/swap/math#Value"/>
        <rdfs:label>lessThan</rdfs:label>
        <rdfs:range rdf:resource="http://www.w3.org/2000/10/swap/math#Value"/>
    </StrictProperty>

    <Function rdf:about="http://www.w3.org/2000/10/swap/math#memberCount">
        <rdfs:comment>The number of items in a list. The subject is a list,
the object is calculated as the number of members.</rdfs:comment>
        <rdfs:domain rdf:resource="http://www.w3.org/2000/10/swap/math#List"/>
        <rdfs:label>memberCount</rdfs:label>
        <rdfs:range rdf:resource="http://www.w3.org/2000/10/swap/math#Value"/>
    </Function>

    <rdf:Property rdf:about="http://www.w3.org/2000/10/swap/math#negation">
        <rdfs:comment>The subject or object is calculated to be the negation of the other.</rdfs:comment>
        <rdfs:domain rdf:resource="http://www.w3.org/2000/10/swap/math#Value"/>
        <rdfs:label>negation</rdfs:label>
        <rdfs:range rdf:resource="http://www.w3.org/2000/10/swap/math#Value"/>
    </rdf:Property>

    <Function rdf:about="http://www.w3.org/2000/10/swap/math#negationOf">
        <rdf:type rdf:resource="http://www.w3.org/2000/10/swap/math#ReverseFunction"/>
        <rdfs:comment>The subject is the negotation of the object (obsolete)</rdfs:comment>
        <rdfs:domain rdf:resource="http://www.w3.org/2000/10/swap/math#Value"/>
        <rdfs:label>negation</rdfs:label>
        <rdfs:range rdf:resource="http://www.w3.org/2000/10/swap/math#Value"/>
    </Function>

    <StrictProperty rdf:about="http://www.w3.org/2000/10/swap/math#notEqualTo">
        <rdfs:comment>True iff the subject is a string representation of a number which  is NOT EQUAL to a number of which the object is a string representation.</rdfs:comment>
        <rdfs:domain rdf:resource="http://www.w3.org/2000/10/swap/math#Value"/>
        <rdfs:label>notEqualTo</rdfs:label>
        <rdfs:range rdf:resource="http://www.w3.org/2000/10/swap/math#Value"/>
    </StrictProperty>

    <StrictProperty rdf:about="http://www.w3.org/2000/10/swap/math#notGreaterThan">
        <rdfs:comment>True iff the subject is a string representation of a number which is NOT greater than the number of which the object is a string representation.</rdfs:comment>
        <rdfs:domain rdf:resource="http://www.w3.org/2000/10/swap/math#Value"/>
        <rdfs:label>notGreaterThan</rdfs:label>
        <rdfs:range rdf:resource="http://www.w3.org/2000/10/swap/math#Value"/>
    </StrictProperty>

    <StrictProperty rdf:about="http://www.w3.org/2000/10/swap/math#notlessThan">
        <rdfs:comment>True iff the subject is a string representation of a number which  is NOT LESS than a number of which the object is a string representation.</rdfs:comment>
        <rdfs:domain rdf:resource="http://www.w3.org/2000/10/swap/math#Value"/>
        <rdfs:label>notlessThan</rdfs:label>
        <rdfs:range rdf:resource="http://www.w3.org/2000/10/swap/math#Value"/>
        <rdfs:subPropertyOf rdf:resource="http://www.w3.org/2000/10/swap/string#notlessThan"/>
    </StrictProperty>

    <rdf:Property rdf:about="http://www.w3.org/2000/10/swap/math#product">
        <rdfs:comment>The subject is a list of numbers.
The object is calculated as the arithmentic product of those numbers.
</rdfs:comment>
        <rdfs:label>product</rdfs:label>
        <rdfs:range rdf:resource="http://www.w3.org/2000/10/swap/math#Value"/>
    </rdf:Property>

    <ReverseFunction rdf:about="http://www.w3.org/2000/10/swap/math#quotientOf">
        <rdfs:comment>The quotient of the list members (obsolete)</rdfs:comment>
        <rdfs:domain rdf:resource="http://www.w3.org/2000/10/swap/math#Value"/>
        <rdfs:label>quotientOf</rdfs:label>
        <rdfs:range rdf:resource="http://www.w3.org/2000/10/swap/math#TwoMemberedList"/>
    </ReverseFunction>

    <ReverseFunction rdf:about="http://www.w3.org/2000/10/swap/math#remainderOf">
        <rdfs:comment>The remainder of the list members (obsolete)</rdfs:comment>
        <rdfs:domain rdf:resource="http://www.w3.org/2000/10/swap/math#Value"/>
        <rdfs:label>remainderOf</rdfs:label>
        <rdfs:range rdf:resource="http://www.w3.org/2000/10/swap/math#TwoMemberedList"/>
    </ReverseFunction>

    <rdf:Property rdf:about="http://www.w3.org/2000/10/swap/math#rounded">
        <rdfs:comment>The object is calulated as the subject rounded to the nearest integer.</rdfs:comment>
        <rdfs:domain rdf:resource="http://www.w3.org/2000/10/swap/math#Value"/>
        <rdfs:label>rounded</rdfs:label>
        <rdfs:range rdf:resource="http://www.w3.org/2000/10/swap/math#Value"/>
    </rdf:Property>

    <rdf:Property rdf:about="http://www.w3.org/2000/10/swap/math#sum">
        <rdfs:comment>The subject is a list of numbers.
The object is calculated as the arithmentic sum of those numbers.
</rdfs:comment>
        <rdfs:label>sum</rdfs:label>
        <rdfs:range rdf:resource="http://www.w3.org/2000/10/swap/math#Value"/>
    </rdf:Property>
</rdf:RDF>
