#Processed by Id: cwm.py,v 1.96 2002/06/07 20:07:17 timbl Exp 
        #    using base file:/devel/WWW/2000/10/swap/time.n3
        
#  Notation3 generation by
#       notation3.py,v 1.108 2002/05/15 00:38:10 timbl Exp

#   Base was: file:/devel/WWW/2000/10/swap/time.n3
     @prefix : <http://www.w3.org/2000/10/swap/time#> .
     @prefix doc: <http://www.w3.org/2000/01/pim/doc#> .
     @prefix log: <http://www.w3.org/2000/10/swap/log#> .
     @prefix ont: <http://www.daml.org/2000/10/daml-ont#> .
     @prefix rdf: <http://www.w3.org/1999/02/22-rdf-syntax-ns#> .
     @prefix rdfs: <http://www.w3.org/2000/01/rdf-schema#> .
    
    :ISOTime     a rdfs:Class .
    
    :day     a ont:UniqueProperty,
                rdf:Property;
         rdfs:comment """
For a date-time, its time:inSeconds is the (string represntation of)
the two-digitday of the month.

Cwm implements this as a function.
""";
         rdfs:domain :ISOTime;
         rdfs:isDefinedBy <>;
         rdfs:label "day" .
    
    :dayOfWeek     a ont:UniqueProperty,
                rdf:Property;
         rdfs:comment """
For a date-time, its time:dayOfWeek is the (string reopresntation of)
the day number within the week, Sunday being 0.

Currently the result is a sinbgle digit string but don't count on it
being anything other than a valid integer represetnation.

Cwm implements this as a function.
""";
         rdfs:domain :ISOTime;
         rdfs:isDefinedBy <>;
         rdfs:label "day of week" .
    
    :gmTime     a ont:UniqueProperty,
                rdf:Property;
         rdfs:comment """
For a date-time format string, its time:gmtime is the 
result of formatting the Universal Time of processing
in the format given.   If teh fiormat string has zero length,
then the ISOdate standrad format is used. 
[ is time:gmtime of ""]  the therefore the current date time.
It will end with "Z" as a timezone code.

Cwm implements this as a function.
""";
         rdfs:isDefinedBy <>;
         rdfs:label "Universal Time";
         rdfs:range :format .
    
    :hour     a ont:UniqueProperty,
                rdf:Property;
         rdfs:comment """
For a date-time, its time:inSeconds is the two-digit hour in the 24 hour clock.

Cwm implements this as a function.
""";
         rdfs:domain :ISOTime;
         rdfs:isDefinedBy <>;
         rdfs:label "hour" .
    
    :inSeconds     a ont:UnambiguousProperty,
                ont:UniqueProperty,
                rdf:Property;
         rdfs:comment """
For a date-time, its time:inSeconds is the (string reopresntation of)
the floating point number of seconds since the beginning of the era
on the given system. Don't assume a particular value, always test for it.

Cwm implements this as a bidirectional function: you can calculae the
ISO date from the seconds since the beginning of the era, or vice-versa.
""";
         rdfs:domain :ISOTime;
         rdfs:isDefinedBy <>;
         rdfs:label "in era seconds" .
    
    :minute     a ont:UniqueProperty,
                rdf:Property;
         rdfs:comment """
For a date-time, its time:minute is the two-digit number of seconds.

Cwm implements this as a function.
""";
         rdfs:domain :ISOTime;
         rdfs:isDefinedBy <>;
         rdfs:label "minute" .
    
    :month     a ont:UniqueProperty,
                rdf:Property;
         rdfs:comment """
For a date-time, its time:inSeconds is the two-digit month.

Cwm implements this as a function.
""";
         rdfs:domain :ISOTime;
         rdfs:isDefinedBy <>;
         rdfs:label "month" .
    
    :second     a ont:UniqueProperty,
                rdf:Property;
         rdfs:comment """
For a date-time, its time:second is the two-digit number of seconds.
Cwm implements this as a function.
""";
         rdfs:domain :ISOTime;
         rdfs:isDefinedBy <>;
         rdfs:label "second" .
    
    :timeZone     a ont:UniqueProperty,
                rdf:Property;
         rdfs:comment """
For a date-time, its time:timeZone is the trailing timezone offset
part, e.g.  "-05:00".
Cwm implements this as a function.
""";
         rdfs:domain :ISOTime;
         rdfs:isDefinedBy <>;
         rdfs:label "timezone offset" .
    
    :year     a ont:UniqueProperty,
                rdf:Property;
         rdfs:comment """
For a date-time, its time:inSeconds is the (string reopresntation of)
the four-digit year.

Cwm implements this as a function.
""";
         rdfs:domain :ISOTime;
         rdfs:isDefinedBy <>;
         rdfs:label "year" .
    
#ENDS
